\documentclass[12pt]{article}
\usepackage[utf8]{inputenc}
\usepackage{latexsym,amsfonts,amssymb,amsthm,amsmath}
\usepackage{float}
\usepackage{caption}
\usepackage{marginnote}
\usepackage{tikz}
\usepackage{hyperref}

\setlength{\parindent}{0in}
\setlength{\oddsidemargin}{0in}
\setlength{\textwidth}{6.5in}
\setlength{\textheight}{8.8in}
\setlength{\topmargin}{0in}
\setlength{\headheight}{18pt}

\newtheorem*{answer*}{Answer}
\newtheorem*{solution*}{Solution}
\newtheorem{remark}{Remark}

\title{Weekly Homework 24}
\author{Math Gecs}
\date{August 15, 2024}

\begin{document}
\maketitle

\subsection*{Exercise 1}
Find all pairs of positive integers $(x,y)$ such that\[x^y = y^{x - y}.\]

Source: 1998 JBMO Problem 3\\

\begin{solution*}
Note that $x^y$ is at least one. Then $y^{x - y}$ is at least one, so $x \geq y$.
\\ \\
Write $x = a^{b+c}, y = a^c$, where $\gcd(b, c) = 1$. (We know that $b$ is nonnegative because $x\geq y$.) Then our equation becomes $a^{(b+c)*a^c} = a^{c*(a^{b+c} - a^c)}$. Taking logarithms base $a$ and dividing through by $a^c$, we obtain $b + c = c*(a^b - 1)$.
\\ \\
Since $c$ divides the RHS of this equation, it must divide the LHS. Since $\gcd(b, c) = 1$ by assumption, we must have $c = 1$, so that the equation reduces to $b + 1 = a^b - 1$, or $b + 2 = a^b$. This equation has only the solutions $b = 1, a = 3$ and $b = 2, a = 2$.
\\ \\
Therefore, our only solutions are $x = 3^{1 + 1} = 9, y = 3^1 = 3$, and $x = 2^{2+1} = 8, y = 2^1 = 2$, and we are done.
\end{solution*}

\end{document}